examples/fs/FSTypes.s.dfy
@@ -1,0 +1,61 @@
+// Copyright 2018-2021 VMware, Inc., Microsoft Inc., Carnegie Mellon University, ETH Zurich, and University of Washington
+// SPDX-License-Identifier: BSD-2-Clause
+
+include "PathSpec.s.dfy"
+include "../../lib/Base/Option.s.dfy"
+
+module FSTypes {
+  import opened NativeTypes
+  import opened Options
+  import opened PathSpec
+
+  type Data = seq<byte>
+
+  datatype FileType = 
+    | File
+    | Directory
+    | SymLink(source: Path)
+    | CharFile(major: int, minor: int) // device identifier
+    | BlockFile(major: int, minor: int) // device identifier
+    | FIFOFile
+    | SocketFile
+
+  datatype Time = Time(seconds: int, nanoseconds: int)
+
+  // metadata tracked by filesys
+  datatype MetaData = MetaData(
+    nlink: int,       // number of hard links
+    size: int,        // size of file
+    ftype: FileType,  // type of file
+    perm: int,        // permission
+    uid: int,         // user ID
+    gid: int,         // group ID
+    atime: Time,      // last accessed time
+    mtime: Time,      // last modified tme 
+    ctime: Time       // last status change time
+  )
+
+  predicate ValidNewMetaData(m: MetaData)
+  {
+    && m.atime == m.ctime == m.mtime
+    && m.size == 0
+    && m.nlink == 1
+  }
+
+  function EmptyMetaData(): MetaData
+  {
+    MetaData(0, 0, File, 0, 0, 0, Time(0,0), Time(0,0), Time(0,0))
+  }
+
+  function InitRootMetaData(): MetaData
+  {
+    MetaData(1, 0, Directory, 755, 0, 0, Time(0,0), Time(0,0), Time(0,0))
+  }
+
+  function EmptyData(): Data
+  {
+    []
+  }
+
+  datatype DirEntry = DirEntry(id: int, path: Path, ftype: FileType)
+}
