examples/fs/PathSpec.s.dfy
@@ -1,0 +1,68 @@
+// Copyright 2018-2021 VMware, Inc., Microsoft Inc., Carnegie Mellon University, ETH Zurich, and University of Washington
+// SPDX-License-Identifier: BSD-2-Clause
+
+include "../../lib/Lang/NativeTypes.s.dfy"
+
+module PathSpec {
+  import opened NativeTypes
+
+  const RootDir :=  ['/' as byte];
+  const RootId := 0;
+  const DefaultId := -1;
+  
+  type Path = seq<byte>
+  type PathMap = imap<Path, int>
+
+  predicate PathComplete(path_map: PathMap)
+  {
+    && (forall path :: path in path_map)
+  }
+
+  function InitPathMap(): (path_map: PathMap)
+  {
+    imap path :: if path == RootDir then RootId else DefaultId
+  }
+
+  predicate InDir(dir: Path, path: Path)
+  {
+    && path != dir
+    && |path| > |dir|
+    && path[..|dir|] == dir
+    && path[|dir|] as int == '/' as int
+  }
+
+  predicate IsEmptyDir(path_map: PathMap, dir: Path)
+  requires PathComplete(path_map)
+  {
+    && (forall k | InDir(dir, k) :: path_map[k] == DefaultId)
+  }
+
+  predicate IsDirEntry(dir: Path, path: Path)
+  {
+    && InDir(dir, path)
+    && !(exists p :: InDir(dir, p) && InDir(p, path))
+    // && (forall i | |dir| < i < |path| :: path[i] as int != '/' as int) // equivalent
+  }
+
+  function GetParentDir(path: Path): (dir: Path)
+  {
+    if |path| == 0 then path
+    else if path[|path|-1] as int == '/' as int then path[..|path|-1]
+    else GetParentDir(path[..|path|-1])
+  }
+
+  predicate ValidPath(path_map: PathMap, path: Path)
+  requires PathComplete(path_map)
+  {
+    && path_map[path] != DefaultId
+  }
+
+  predicate ValidNewPath(path_map: PathMap, path: Path)
+  requires PathComplete(path_map)
+  {
+    var parentdir := GetParentDir(path);
+    && ValidPath(path_map, parentdir)
+    && IsDirEntry(parentdir, path)
+    && path_map[path] == DefaultId
+  }
+}
